lio_proofs.v
@@ -57,25 +57,25 @@ Qed.
 
 Hint Resolve values_cannot_be_lio_reduced.
 
-Theorem deterministic_pure_reduce :
+Lemma deterministic_pure_reduce :
   deterministic pure_reduce.
 Proof.
   unfold deterministic. intros x y1 y2 Hy1 Hy2.
   generalize dependent y2. 
   pure_reduce_cases (induction Hy1) Case; intros y2 Hy2.
   Case "Pr_appCtx". inversion Hy2. 
-   SCase "Pr_appCtx". apply IHHy1 in H8. subst. reflexivity.
+   SCase "Pr_appCtx". apply IHHy1 in H2. subst. reflexivity.
    SCase "Pr_app". subst t3. subst. solve by inversion. 
   Case "Pr_app". inversion Hy2. subst t3. solve by inversion.  reflexivity.
-  Case "Pr_fixCtx". inversion Hy2. subst t5. apply IHHy1 in H4. subst t'0. reflexivity.
+  Case "Pr_fixCtx". inversion Hy2. subst t5. apply IHHy1 in H0. subst t'0. reflexivity.
     subst. inversion Hy1.
-  Case "Pr_fix". inversion Hy2.  inversion H3. reflexivity.
-  Case "Pr_ifCtx". inversion Hy2. apply IHHy1 in H11. subst. reflexivity. 
+  Case "Pr_fix". inversion Hy2.  solve by inversion. reflexivity.
+  Case "Pr_ifCtx". inversion Hy2. apply IHHy1 in H3. subst. reflexivity. 
    SCase "true". subst. inversion Hy1.
    SCase "false". subst. inversion Hy1.
   Case "Pr_ifTrue". inversion Hy2. solve by inversion. reflexivity.
   Case "Pr_ifFalse". inversion Hy2. solve by inversion. reflexivity.
-  Case "Pr_joinCtxL". inversion Hy2. subst t3 t1. apply IHHy1 in H8. subst t1'0. reflexivity.
+  Case "Pr_joinCtxL". inversion Hy2. subst t3 t1. apply IHHy1 in H2. subst t1'0. reflexivity.
    subst t2 t1. apply labels_cannot_be_reduced in Hy1. solve by inversion. assumption.
    subst. apply labels_cannot_be_reduced in Hy1. solve by inversion. reflexivity.
    subst t1 y2. apply labels_cannot_be_reduced in Hy1. solve by inversion. assumption.
@@ -84,8 +84,8 @@ Proof.
    subst.  apply labels_cannot_be_reduced in Hy1. solve by inversion. reflexivity.
    subst.  apply labels_cannot_be_reduced in Hy1. solve by inversion. reflexivity.
    subst.  apply labels_cannot_be_reduced in Hy1. solve by inversion. assumption.
-  Case "Pr_joinCtxR". inversion Hy2. apply labels_cannot_be_reduced in H8. solve by inversion. assumption.
-   subst. apply IHHy1 in H8. subst t2'0. reflexivity.
+  Case "Pr_joinCtxR". inversion Hy2. apply labels_cannot_be_reduced in H3. solve by inversion. assumption.
+   subst. apply IHHy1 in H4. subst t2'0. reflexivity.
    subst. apply labels_cannot_be_reduced in Hy1. solve by inversion. assumption.
    subst. apply labels_cannot_be_reduced in Hy1. solve by inversion. simpl. reflexivity. 
    subst. apply labels_cannot_be_reduced in Hy1. solve by inversion. simpl. assumption.
@@ -93,20 +93,20 @@ Proof.
    subst. apply labels_cannot_be_reduced in Hy1. solve by inversion. simpl. reflexivity.  
    subst. apply labels_cannot_be_reduced in Hy1. solve by inversion. simpl. assumption.
    subst. apply labels_cannot_be_reduced in Hy1. solve by inversion. simpl. reflexivity. 
-  Case "Pr_joinBotL". inversion Hy2. apply labels_cannot_be_reduced in H7. solve by inversion. reflexivity. 
-   subst. apply labels_cannot_be_reduced in H7. solve by inversion. apply H.
+  Case "Pr_joinBotL". inversion Hy2. apply labels_cannot_be_reduced in H4. solve by inversion. reflexivity. 
+   subst. apply labels_cannot_be_reduced in H5. solve by inversion. assumption. 
    reflexivity.
    reflexivity.
    auto.
    reflexivity.
-  Case "Pr_joinBotR". inversion Hy2. apply labels_cannot_be_reduced in H7. solve by inversion. assumption.
-   subst. apply labels_cannot_be_reduced in H7. solve by inversion. reflexivity.
+  Case "Pr_joinBotR". inversion Hy2. apply labels_cannot_be_reduced in H4. solve by inversion. assumption.
+   subst. apply labels_cannot_be_reduced in H5. solve by inversion. reflexivity.
    reflexivity.
    reflexivity.
    reflexivity.
    reflexivity.
-  Case "Pr_joinEq". inversion Hy2. apply labels_cannot_be_reduced in H8. solve by inversion. assumption.
-   subst. apply labels_cannot_be_reduced in H8. solve by inversion. assumption.
+  Case "Pr_joinEq". inversion Hy2. apply labels_cannot_be_reduced in H5. solve by inversion. assumption.
+   subst. apply labels_cannot_be_reduced in H6. solve by inversion. assumption.
    subst. auto. 
    reflexivity. 
    reflexivity.
@@ -114,28 +114,28 @@ Proof.
    subst. solve by inversion. 
    reflexivity.
    subst. reflexivity.
-  Case "Pr_joinAB". inversion Hy2. apply labels_cannot_be_reduced in H5. solve by inversion. reflexivity.
-   apply labels_cannot_be_reduced in H5. solve by inversion. reflexivity.
+  Case "Pr_joinAB". inversion Hy2. apply labels_cannot_be_reduced in H2. solve by inversion. reflexivity.
+   apply labels_cannot_be_reduced in H3. solve by inversion. reflexivity.
    solve by inversion.
    reflexivity.
    auto.
-  Case "Pr_joinBA". inversion Hy2. apply labels_cannot_be_reduced in H5. solve by inversion. reflexivity.
-   apply labels_cannot_be_reduced in H5. solve by inversion. reflexivity.
+  Case "Pr_joinBA". inversion Hy2. apply labels_cannot_be_reduced in H2. solve by inversion. reflexivity.
+   apply labels_cannot_be_reduced in H3. solve by inversion. reflexivity.
    solve by inversion.
    reflexivity.
-  Case "Pr_joinTopL". inversion Hy2. apply labels_cannot_be_reduced in H7. solve by inversion. reflexivity.
-   apply labels_cannot_be_reduced in H7. inversion H7. assumption.
+  Case "Pr_joinTopL". inversion Hy2. apply labels_cannot_be_reduced in H4. solve by inversion. reflexivity.
+   apply labels_cannot_be_reduced in H5. solve by inversion. assumption.
    reflexivity.
    reflexivity.
    reflexivity.
    reflexivity.
-  Case "Pr_joinTopR". inversion Hy2. apply labels_cannot_be_reduced in H7. solve by inversion. assumption.
-   apply labels_cannot_be_reduced in H7. solve by inversion. reflexivity.
+  Case "Pr_joinTopR". inversion Hy2. apply labels_cannot_be_reduced in H4. solve by inversion. assumption.
+   apply labels_cannot_be_reduced in H5. solve by inversion. reflexivity.
    reflexivity.
    auto.
    reflexivity.
    reflexivity.
-  Case "Pr_meetCtxL". inversion Hy2. subst t3 t1. apply IHHy1 in H8. subst t1'0. reflexivity.
+  Case "Pr_meetCtxL". inversion Hy2. subst t3 t1. apply IHHy1 in H2. subst t1'0. reflexivity.
    subst t2 t1. apply labels_cannot_be_reduced in Hy1. solve by inversion. assumption. 
    subst. apply labels_cannot_be_reduced in Hy1. solve by inversion. reflexivity.
    subst t1 y2. apply labels_cannot_be_reduced in Hy1. solve by inversion. assumption.
@@ -144,8 +144,8 @@ Proof.
    subst.  apply labels_cannot_be_reduced in Hy1. solve by inversion. reflexivity.
    subst.  apply labels_cannot_be_reduced in Hy1. solve by inversion. reflexivity.
    subst.  apply labels_cannot_be_reduced in Hy1. solve by inversion. assumption.
-  Case "Pr_meetCtxR". inversion Hy2. apply labels_cannot_be_reduced in H8. solve by inversion. assumption.
-   subst. apply IHHy1 in H8. subst t2'0. reflexivity.
+  Case "Pr_meetCtxR". inversion Hy2. apply labels_cannot_be_reduced in H3. solve by inversion. assumption.
+   subst. apply IHHy1 in H4. subst t2'0. reflexivity.
    subst. apply labels_cannot_be_reduced in Hy1. solve by inversion. simpl. assumption.
    subst. apply labels_cannot_be_reduced in Hy1. solve by inversion. simpl. reflexivity. 
    subst. apply labels_cannot_be_reduced in Hy1. solve by inversion. simpl. assumption.
@@ -153,20 +153,20 @@ Proof.
    subst. apply labels_cannot_be_reduced in Hy1. solve by inversion. simpl. reflexivity.  
    subst. apply labels_cannot_be_reduced in Hy1. solve by inversion. simpl. assumption.
    subst. apply labels_cannot_be_reduced in Hy1. solve by inversion. simpl. reflexivity. 
-  Case "Pr_meetBotL". inversion Hy2. apply labels_cannot_be_reduced in H7. solve by inversion. reflexivity. 
-   subst. apply labels_cannot_be_reduced in H7. solve by inversion. assumption.
+  Case "Pr_meetBotL". inversion Hy2. apply labels_cannot_be_reduced in H4. solve by inversion. reflexivity. 
+   subst. apply labels_cannot_be_reduced in H5. solve by inversion. assumption.
    reflexivity.
    reflexivity.
    auto.
    reflexivity.
-  Case "Pr_meetBotR". inversion Hy2. apply labels_cannot_be_reduced in H7. solve by inversion. assumption.
-   subst. apply labels_cannot_be_reduced in H7. solve by inversion. reflexivity.
+  Case "Pr_meetBotR". inversion Hy2. apply labels_cannot_be_reduced in H4. solve by inversion. assumption.
+   subst. apply labels_cannot_be_reduced in H5. solve by inversion. reflexivity.
    reflexivity.
    reflexivity.
    auto.
    reflexivity.
-  Case "Pr_meetEq". inversion Hy2. apply labels_cannot_be_reduced in H8. solve by inversion. assumption.
-   subst. apply labels_cannot_be_reduced in H8. solve by inversion. assumption.
+  Case "Pr_meetEq". inversion Hy2. apply labels_cannot_be_reduced in H5. solve by inversion. assumption.
+   subst. apply labels_cannot_be_reduced in H6. solve by inversion. assumption.
    subst. auto. 
    subst. reflexivity. 
    reflexivity.
@@ -174,79 +174,80 @@ Proof.
    subst. solve by inversion.
    subst. auto.
    reflexivity.
-  Case "Pr_meetAB". inversion Hy2. apply labels_cannot_be_reduced in H5. solve by inversion. reflexivity.
-   apply labels_cannot_be_reduced in H5. solve by inversion. reflexivity.
+  Case "Pr_meetAB". inversion Hy2. apply labels_cannot_be_reduced in H2. solve by inversion. reflexivity.
+   apply labels_cannot_be_reduced in H3. solve by inversion. reflexivity.
    solve by inversion.
    reflexivity.
-  Case "Pr_meetBA". inversion Hy2. apply labels_cannot_be_reduced in H5. solve by inversion. reflexivity.
-   apply labels_cannot_be_reduced in H5. solve by inversion. reflexivity.
+  Case "Pr_meetBA". inversion Hy2. apply labels_cannot_be_reduced in H2. solve by inversion. reflexivity.
+   apply labels_cannot_be_reduced in H3. solve by inversion. reflexivity.
    solve by inversion.
    reflexivity.
-  Case "Pr_meetTopL". inversion Hy2. apply labels_cannot_be_reduced in H7. solve by inversion. reflexivity.
-   apply labels_cannot_be_reduced in H7. solve by inversion. assumption.
+  Case "Pr_meetTopL". inversion Hy2. apply labels_cannot_be_reduced in H4. solve by inversion. reflexivity.
+   apply labels_cannot_be_reduced in H5. solve by inversion. assumption.
    reflexivity.
    subst. auto. 
    reflexivity.
    reflexivity.
-  Case "Pr_meetTopR". inversion Hy2. apply labels_cannot_be_reduced in H7. solve by inversion. assumption.
-   apply labels_cannot_be_reduced in H7. solve by inversion. reflexivity.
+  Case "Pr_meetTopR". inversion Hy2. apply labels_cannot_be_reduced in H4. solve by inversion. assumption.
+   apply labels_cannot_be_reduced in H5. solve by inversion. reflexivity.
    reflexivity.
    reflexivity.
    reflexivity.
    reflexivity.
-  Case "Pr_canFlowToCtxL". inversion Hy2. subst t3 t1. apply IHHy1 in H8. subst t1'0. reflexivity.
+  Case "Pr_canFlowToCtxL". inversion Hy2. subst t3 t1. apply IHHy1 in H2. subst t1'0. reflexivity.
    subst t2 t1. apply labels_cannot_be_reduced in Hy1. solve by inversion. assumption.
    subst. apply labels_cannot_be_reduced in Hy1. solve by inversion. reflexivity.
    subst t1 y2. apply labels_cannot_be_reduced in Hy1. solve by inversion. assumption.
    subst.  apply labels_cannot_be_reduced in Hy1. solve by inversion. reflexivity.
    subst.  apply labels_cannot_be_reduced in Hy1. solve by inversion. reflexivity.
    subst.  apply labels_cannot_be_reduced in Hy1. solve by inversion. assumption.
-  Case "Pr_canFlowToCtxR". inversion Hy2. apply labels_cannot_be_reduced in H8. solve by inversion. assumption.
-   subst. apply IHHy1 in H8. subst t2'0. reflexivity.
+  Case "Pr_canFlowToCtxR". inversion Hy2. apply labels_cannot_be_reduced in H3. solve by inversion. assumption.
+   subst. apply IHHy1 in H4. subst t2'0. reflexivity.
    subst. apply labels_cannot_be_reduced in Hy1. solve by inversion. assumption.
    subst. apply labels_cannot_be_reduced in Hy1. solve by inversion. simpl. assumption.
    subst. apply labels_cannot_be_reduced in Hy1. solve by inversion. simpl. trivial.
    subst. apply labels_cannot_be_reduced in Hy1. solve by inversion. simpl. trivial.
    subst. apply labels_cannot_be_reduced in Hy1. solve by inversion. simpl. trivial.
-  Case "Pr_canFlowToBot". inversion Hy2. apply labels_cannot_be_reduced in H7. solve by inversion. reflexivity. 
-   subst. apply labels_cannot_be_reduced in H7. solve by inversion. assumption.
+  Case "Pr_canFlowToBot". inversion Hy2. apply labels_cannot_be_reduced in H4. solve by inversion. reflexivity. 
+   subst. apply labels_cannot_be_reduced in H5. solve by inversion. assumption.
    reflexivity.
    reflexivity.
    auto.
-  Case "Pr_canFlowToEq". inversion Hy2. apply labels_cannot_be_reduced in H8. solve by inversion. assumption.
-   subst. apply labels_cannot_be_reduced in H8. solve by inversion. assumption.
+  Case "Pr_canFlowToEq". inversion Hy2. apply labels_cannot_be_reduced in H5. solve by inversion. assumption.
+   subst. apply labels_cannot_be_reduced in H6. solve by inversion. assumption.
    subst. auto. 
    subst. reflexivity. 
    subst. solve by inversion.
    subst. solve by inversion.
    subst. reflexivity.
-  Case "Pr_canFlowToAB". inversion Hy2. apply labels_cannot_be_reduced in H5. solve by inversion. reflexivity.
-   apply labels_cannot_be_reduced in H5. solve by inversion. reflexivity.
+  Case "Pr_canFlowToAB". inversion Hy2. apply labels_cannot_be_reduced in H2. solve by inversion. reflexivity.
+   apply labels_cannot_be_reduced in H3. solve by inversion. reflexivity.
    solve by inversion.
    reflexivity.
-  Case "Pr_canFlowToBA". inversion Hy2. apply labels_cannot_be_reduced in H5. solve by inversion. reflexivity.
-   apply labels_cannot_be_reduced in H5. solve by inversion. reflexivity.
+  Case "Pr_canFlowToBA". inversion Hy2. apply labels_cannot_be_reduced in H2. solve by inversion. reflexivity.
+   apply labels_cannot_be_reduced in H3. solve by inversion. reflexivity.
    solve by inversion.
    reflexivity.
-  Case "Pr_canFlowToTop". inversion Hy2. apply labels_cannot_be_reduced in H7. solve by inversion. assumption.
-   apply labels_cannot_be_reduced in H7. solve by inversion. reflexivity.
+  Case "Pr_canFlowToTop". inversion Hy2. apply labels_cannot_be_reduced in H4. solve by inversion. assumption.
+   apply labels_cannot_be_reduced in H5. solve by inversion. reflexivity.
    reflexivity.
    reflexivity.
    reflexivity.
-  Case "Pr_labelOfCtx". inversion Hy2. subst. apply IHHy1 in H4. subst t'0. reflexivity.
-    subst. apply values_cannot_be_reduced in Hy1. solve by inversion. trivial.
+  Case "Pr_labelOfCtx". inversion Hy2. subst. apply IHHy1 in H0. subst t'0. reflexivity.
+    subst. apply values_cannot_be_reduced in Hy1. solve by inversion. simpl. trivial.
   Case "Pr_labelOf". inversion Hy2. 
-    subst. inversion H5. reflexivity.
+    subst. solve by inversion. reflexivity.
 Qed.
 
 Hint Resolve deterministic_pure_reduce.
-
 
 Axiom alpha_equiv_abs_mkTo : forall l c t x x' l' c' l1,
   m_Config l c (t_Bind t (t_VAbs x  (t_MkToLabeledTCB l' c' l1 (t_Var x )))) =
   m_Config l c (t_Bind t (t_VAbs x' (t_MkToLabeledTCB l' c' l1 (t_Var x')))).
 
-Theorem deterministic_lio_reduce :
+Hint Resolve alpha_equiv_abs_mkTo.
+
+Lemma deterministic_lio_reduce :
   deterministic lio_reduce.
 Proof.
   unfold deterministic. intros x y1 y2 Hy1 Hy2.
@@ -256,13 +257,13 @@ Proof.
     inversion Hy2. reflexivity.
   Case "LIO_bindCtx".
     inversion Hy2.
-    subst. apply IHHy1 in H14. inversion H14. reflexivity.
+    subst. apply IHHy1 in H8. inversion H8. reflexivity.
     subst.
     inversion Hy2.
     subst. inversion Hy1. 
   Case "LIO_bind".
     inversion Hy2.
-    subst. inversion H12. reflexivity.
+    subst. inversion H7. reflexivity.
   Case "LIO_getLabel".
     inversion Hy2.
     subst. reflexivity.
@@ -276,11 +277,11 @@ Proof.
     SCase "assertion". apply  deterministic_pure_reduce with (x := t1). assumption. assumption.
     subst t1'0. reflexivity.
     subst t1 c0 l_5 t2.
-    apply labels_cannot_be_reduced in H3. solve by inversion. assumption.
+    apply labels_cannot_be_reduced in H0. solve by inversion. assumption.
   Case "LIO_label".
     inversion Hy2.
     subst. 
-    apply labels_cannot_be_reduced in H16. solve by inversion. assumption.
+    apply labels_cannot_be_reduced in H. solve by inversion. assumption.
     reflexivity.
   Case "LIO_unlabelCtx".
     inversion Hy2.
@@ -289,11 +290,11 @@ Proof.
     SCase "assertion". apply  deterministic_pure_reduce with (x := t5). assumption. assumption.
     subst t'0. reflexivity.
     subst. 
-    apply values_cannot_be_reduced in H2. solve by inversion. trivial.
+    apply values_cannot_be_reduced in H0. solve by inversion. trivial.
  Case "LIO_unlabel".
     inversion Hy2.
     subst.
-    apply values_cannot_be_reduced in H16. solve by inversion. trivial.
+    apply values_cannot_be_reduced in H12. solve by inversion. trivial.
     subst.
     assert (l2 = l3).
     SCase "assertion". apply deterministic_pure_reduce with (x := t_Join l_5 l1). assumption. assumption.
@@ -307,18 +308,66 @@ Proof.
     reflexivity.
 Qed.
 
-Definition canFlowTo (l1 l2 :t) : bool :=
-  match l1, l2 with
-    | t_LBot , _      => true
-    | _      , t_LTop => true
-    | t_LA   , t_A    => true
-    | t_LB   , t_B    => true
-    | _      , _      => false
+Hint Resolve deterministic_lio_reduce.
+
+Definition isLabel (t_6:t) : bool :=
+  match t_6 with
+  | t_LBot => (true)
+  | t_LA => (true)
+  | t_LB => (true)
+  | t_LTop => (true)
+  | _ => false
+end.
+
+Lemma isLabel_is_l_of_t : forall term,
+  isLabel term = true <-> is_l_of_t term.
+Proof.
+  intros.
+  induction term; simpl; eauto; try split; try reflexivity; try split; intros; try solve by inversion.
+Qed.
+
+Definition canFlowTo (l1 l2 :t) : option bool :=
+  match l1 with
+    | t_LBot =>  match l2 with
+                 | t_LBot  => Some true
+                 | t_LA    => Some true
+                 | t_LB    => Some true
+                 | t_LTop  => Some true
+                 | _       => None
+                 end
+    | t_LA    =>  match l2 with
+                 | t_LBot  => Some false
+                 | t_LA     => Some true
+                 | t_LB     => Some false
+                 | t_LTop  => Some true
+                 | _       => None
+                 end
+    | t_LB    =>  match l2 with
+                 | t_LBot  => Some false
+                 | t_LA     => Some false
+                 | t_LB     => Some true
+                 | t_LTop  => Some true
+                 | _       => None
+                 end
+    | t_LTop =>  match l2 with
+                 | t_LBot  => Some false
+                 | t_LA     => Some false
+                 | t_LB     => Some false
+                 | t_LTop  => Some true
+                 | _       => None
+                 end
+    | _       => None
   end.
 
-Notation " l1  '[=' l2 " := (canFlowTo l1 l2) (at label 40).    
+Definition eq_option_bool (o1 o2 : option bool) : bool :=
+  match o1, o2 with
+    | Some x , Some y => eqb x y
+    | _, _ => false
+  end.
 
-Fixpoint erase (l term : t) : t :=
+Notation " o1 '===' o2 " := (eq_option_bool o1 o2) (at level 40).
+
+Fixpoint erase_term (l term : t) : t :=
   match term with
    | t_LBot            => t_LBot
    | t_LA              => t_LA
@@ -327,25 +376,356 @@ Fixpoint erase (l term : t) : t :=
    | t_VTrue           => t_VTrue
    | t_VFalse          => t_VFalse
    | t_VUnit           => t_VUnit
-   | t_VAbs x t5       => t_VAbs x (erase l t5)
-   | t_VFix t5         => t_VFix (erase l t5)
-   | t_VLIO t5         => t_VFix (erase l t5)
-   | t_VLabeled l1 t2  => if l1 [= l
-                           then t_VLabeled (erase l l1) (if l1 [= l then erase l t2) else hole
+   | t_VAbs x t5       => t_VAbs x (erase_term l t5)
+   | t_VFix t5         => t_VFix (erase_term l t5)
+   | t_VLIO t5         => t_VFix (erase_term l t5)
+   | t_VLabeled l1 t2  => t_VLabeled l1 (if canFlowTo l1 l === Some true
+                                           then erase_term l t2
+                                           else t_VHole)
    | t_VHole           => t_VHole
    | t_Var x           => t_Var x
-   | t_App t5 t'       => t_App (erase l t5) (erase l t')
-   | t_IfEl t1 t2 t3   => t_IfEl (erase l t1) (erase l t2) (erase l t3)
-   | t_Join t1 t2      => t_Join (erase l t1) (erase l t2)
-   | t_Meet t1 t2      => t_Meet (erase l t1) (erase l t2)
-   | t_CanFlowTo t1 t2 => t_CanFlowTo (erase l t1) (erase l t2)
-   | t_Return t5       => t_Return (erase l t5)
-   | t_Bind t5 t'      => t_Bind (erase l t5) (erase l t')
+   | t_App t5 t'       => t_App (erase_term l t5) (erase_term l t')
+   | t_IfEl t1 t2 t3   => t_IfEl t1 (erase_term l t2) (erase_term l t3)
+   | t_Join t1 t2      => t_Join t1 t2
+   | t_Meet t1 t2      => t_Meet t1 t2
+   | t_CanFlowTo t1 t2 => t_CanFlowTo t1 t2
+   | t_Return t5       => t_Return (erase_term l t5)
+   | t_Bind t5 t'      => t_Bind (erase_term l t5) (erase_term l t')
    | t_GetLabel        => t_GetLabel
    | t_GetClearance    => t_GetClearance
-   | t_LabelOf t5      => t_LabelOf (erase l t5)
-   | t_Label t5 t'     => t_Label (erase l t5) (erase l t')
-   | t_UnLabel t5      => t_UnLabel (erase l t5)
-   | t_ToLabeled t1 t2 =>  t_ToLabeled (erase l t1) (erase l t2)
-   | t_MkToLabeledTCB l_5 c l1 t5 => t_MkToLabeledTCB (erase l l_5) (erase l c) (erase l l1) (erase l t5)
+   | t_LabelOf t5      => t_LabelOf (erase_term l t5)
+   | t_Label t5 t'     => t_Label t5 (erase_term l t')
+   | t_UnLabel t5      => t_UnLabel (erase_term l t5)
+   | t_ToLabeled t1 t2 => t_ToLabeled t1 (erase_term l t2)
+   | t_MkToLabeledTCB l_5 c l1 t5 => t_MkToLabeledTCB l_5 c l1 (erase_term l t5)
   end.
+
+Inductive erase_term_inv : t -> t -> t -> Prop :=
+  | erase_term_inv_t_VAbs : forall l t5,
+     t_VAbs x (erase_term l t5) -> erase_term l (t_VAbs x t5)
+  | erase_term_inv_t_VFix : forall l t5,
+     t_VFix (erase_term l t5) -> erase_term l (t_VFix t5)
+  | erase_term_inv_t_VLIO : forall l t5,
+     t_VFix (erase_term l t5) -> erase_term l (t_VLIO t5)
+  | erase_term_inv_t_VLabeled1 : forall l l1 t2,
+    t_VLabeled l1 (erase_term l t2) -> erase_term l (t_VLabeled l1 t2)
+(*
+  | t_VLabeled l1 t2  => t_VLabeled l1 (if canFlowTo l1 l === Some true
+                                           then erase_term l t2
+                                           else t_VHole)
+*)
+   | erase_term_inv_t_VHole : forall l t1,
+     t_VHole -> erase_term l t1
+   | ersae_term_inv_t_App : forall l t5 t',
+     t_App (erase_term l t5) (erase_term l t') -> erase_temr l (t_App t5 t')
+   | t_IfEl t1 t2 t3   => t_IfEl t1 (erase_term l t2) (erase_term l t3)
+   | t_Join t1 t2      => t_Join t1 t2
+   | t_Meet t1 t2      => t_Meet t1 t2
+   | t_CanFlowTo t1 t2 => t_CanFlowTo t1 t2
+   | t_Return t5       => t_Return (erase_term l t5)
+   | t_Bind t5 t'      => t_Bind (erase_term l t5) (erase_term l t')
+   | t_GetLabel        => t_GetLabel
+   | t_GetClearance    => t_GetClearance
+   | t_LabelOf t5      => t_LabelOf (erase_term l t5)
+   | t_Label t5 t'     => t_Label t5 (erase_term l t')
+   | t_UnLabel t5      => t_UnLabel (erase_term l t5)
+   | t_ToLabeled t1 t2 => t_ToLabeled t1 (erase_term l t2)
+   | t_MkToLabeledTCB l_5 c l1 t5 => t_MkToLabeledTCB l_5 c l1 (erase_term l t5)
+
+(* ~>L *)
+Inductive pure_reduce_l : t -> t -> t -> Prop :=
+   | pure_reduce_l_step : forall l t1 t2,
+     is_l_of_t l ->
+     pure_reduce t1 t2 ->
+     pure_reduce_l l t1 (erase_term l t2).
+
+
+Lemma deterministic_pure_reduce_l : forall l x y1 y2,
+  pure_reduce_l l x y1 ->
+  pure_reduce_l l x y2 ->
+  y1 = y2.
+Proof.
+  intros l x y1 y2 Hy1 Hy2. 
+  generalize dependent y2.
+  induction Hy1; intros y2 Hy2.
+  inversion Hy2.
+  assert (t2 = t3).
+  Case "assertion". apply deterministic_pure_reduce with (x := t1). assumption. assumption.
+  subst t3 t1.
+  reflexivity.
+Qed.
+
+Definition erase_config (l : t) (cfg : m) : m :=
+  match cfg with
+   | m_Config l1 c1 t1 => if canFlowTo l1 l
+                            then m_Config l1 c1 (erase_term l t1)
+                            else m_Config l1 c1 t_VHole
+  end.
+
+(* -->L *)
+Inductive lio_reduce_l : t -> m -> m -> Prop :=
+   | lio_reduce_l_step : forall l m1 m2,
+     is_l_of_t l ->
+     lio_reduce m1 m2 ->
+     lio_reduce_l l m1 m2.
+
+Lemma deterministic_lio_reduce_l : forall l x y1 y2,
+  lio_reduce_l l x y1 ->
+  lio_reduce_l l x y2 ->
+  y1 = y2.
+Proof.
+  intros l x y1 y2 Hy1 Hy2. 
+  generalize dependent y2.
+  induction Hy1; intros y2 Hy2.
+  inversion Hy2.
+  Case "assertion". apply deterministic_lio_reduce with (x := m1). assumption. assumption.
+Qed.
+
+Hint Resolve deterministic_lio_reduce_l.
+
+Lemma erase_term_idempotent : forall l t1,
+  is_l_of_t l ->
+  erase_term l t1 = erase_term l (erase_term l t1).
+Proof.
+  intros l t1 H.
+  term_cases (induction t1) Case; eauto.
+  Case "term_VAbs". simpl. rewrite <- IHt1. reflexivity.
+  Case "term_VFix". simpl. rewrite <- IHt1. reflexivity.
+  Case "term_VLIO". simpl. rewrite <- IHt1. reflexivity.
+  Case "term_VLabeled". induction l; try contradiction.
+    SCase "LBot". simpl.
+     destruct t1_1. simpl. rewrite <- IHt1_2; reflexivity.
+     auto. auto. auto. auto. auto. auto. auto.
+     simpl. inversion IHt1_1. reflexivity.
+     simpl. inversion IHt1_1. reflexivity.
+     simpl. inversion IHt1_1. reflexivity.
+     simpl. inversion IHt1_1. reflexivity.
+     simpl. inversion IHt1_1. reflexivity.
+     auto.
+     auto.
+     simpl. inversion IHt1_1. reflexivity.
+     simpl. inversion IHt1_1. reflexivity.
+     simpl. inversion IHt1_1. reflexivity.
+     simpl. inversion IHt1_1. reflexivity.
+     simpl. inversion IHt1_1. reflexivity.
+     simpl. inversion IHt1_1. reflexivity.
+     simpl. inversion IHt1_1. reflexivity.
+     auto. 
+     auto. 
+     simpl. inversion IHt1_1. reflexivity.
+     simpl. inversion IHt1_1. reflexivity.
+     simpl. inversion IHt1_1. reflexivity.
+    SCase "LA". simpl.
+     destruct t1_1. simpl. rewrite <- IHt1_2; reflexivity.
+     auto. auto. auto. auto. auto. auto. auto.
+     simpl. inversion IHt1_2. reflexivity.
+     simpl. inversion IHt1_1. reflexivity.
+     simpl. inversion IHt1_1. reflexivity.
+     simpl. inversion IHt1_1. reflexivity.
+     simpl. inversion IHt1_1. reflexivity.
+     auto.
+     auto.
+     simpl. inversion IHt1_1. reflexivity.
+     simpl. inversion IHt1_1. reflexivity.
+     simpl. inversion IHt1_1. reflexivity.
+     simpl. inversion IHt1_1. reflexivity.
+     simpl. inversion IHt1_1. reflexivity.
+     simpl. inversion IHt1_1. reflexivity.
+     simpl. inversion IHt1_1. reflexivity.
+     auto. 
+     auto. 
+     simpl. inversion IHt1_1. reflexivity.
+     simpl. inversion IHt1_1. reflexivity.
+     simpl. inversion IHt1_1. reflexivity.
+     simpl. inversion IHt1_1. reflexivity.
+     simpl. inversion IHt1_1. reflexivity.
+     simpl. inversion IHt1_1. reflexivity.
+     simpl. inversion IHt1_1. reflexivity.
+     simpl. inversion IHt1_1. reflexivity.
+     simpl. inversion IHt1_1. reflexivity.
+     simpl. inversion IHt1_1. reflexivity.
+    SCase "LB". simpl.
+     destruct t1_1. simpl. rewrite <- IHt1_2; reflexivity.
+     auto. auto. auto. auto. auto. auto. auto.
+     simpl. inversion IHt1_2. reflexivity.
+     simpl. inversion IHt1_1. reflexivity.
+     simpl. inversion IHt1_1. reflexivity.
+     simpl. inversion IHt1_1. reflexivity.
+     simpl. inversion IHt1_1. reflexivity.
+     auto.
+     auto.
+     simpl. inversion IHt1_1. reflexivity.
+     simpl. inversion IHt1_1. reflexivity.
+     simpl. inversion IHt1_1. reflexivity.
+     simpl. inversion IHt1_1. reflexivity.
+     simpl. inversion IHt1_1. reflexivity.
+     simpl. inversion IHt1_1. reflexivity.
+     simpl. inversion IHt1_1. reflexivity.
+     auto. 
+     auto. 
+     simpl. inversion IHt1_1. reflexivity.
+     simpl. inversion IHt1_1. reflexivity.
+     simpl. inversion IHt1_1. reflexivity.
+     simpl. inversion IHt1_1. reflexivity.
+     simpl. inversion IHt1_1. reflexivity.
+     simpl. inversion IHt1_1. reflexivity.
+     simpl. inversion IHt1_1. reflexivity.
+     simpl. inversion IHt1_1. reflexivity.
+     simpl. inversion IHt1_1. reflexivity.
+    SCase "LTop". simpl.
+     destruct t1_1. simpl. rewrite <- IHt1_2; reflexivity.
+     auto. auto. auto. auto. auto. auto. auto.
+     simpl. inversion IHt1_2. reflexivity.
+     simpl. rewrite <- IHt1_2. reflexivity.
+     simpl. rewrite <- IHt1_2. reflexivity.
+     simpl. inversion IHt1_1. reflexivity.
+     simpl. inversion IHt1_1. reflexivity.
+     auto.
+     auto.
+     simpl. inversion IHt1_1. reflexivity.
+     simpl. inversion IHt1_1. reflexivity.
+     simpl. inversion IHt1_1. reflexivity.
+     simpl. inversion IHt1_1. reflexivity.
+     simpl. inversion IHt1_1. reflexivity.
+     simpl. inversion IHt1_1. reflexivity.
+     simpl. inversion IHt1_1. reflexivity.
+     auto. 
+     auto. 
+     simpl. inversion IHt1_1. reflexivity.
+     simpl. inversion IHt1_1. reflexivity.
+     simpl. inversion IHt1_1. reflexivity.
+     simpl. inversion IHt1_1. reflexivity.
+     simpl. inversion IHt1_1. reflexivity.
+     simpl. inversion IHt1_1. reflexivity.
+     simpl. inversion IHt1_1. reflexivity.
+     simpl. inversion IHt1_1. reflexivity.
+     simpl. inversion IHt1_1. reflexivity.
+     simpl. inversion IHt1_1. reflexivity.
+  Case "term_App". simpl. rewrite <- IHt1_1. rewrite <- IHt1_2. reflexivity.
+  Case "term_IfEl". simpl. rewrite <- IHt1_2. rewrite <- IHt1_3. reflexivity.
+  Case "term_Return". simpl. rewrite <- IHt1. reflexivity.
+  Case "term_Bind". simpl. rewrite <- IHt1_1. rewrite <- IHt1_2. reflexivity.
+  Case "term_LabelOf". simpl. rewrite <- IHt1. reflexivity.
+  Case "term_Label". simpl. rewrite <- IHt1_2. reflexivity.
+  Case "term_UnLabel". simpl. rewrite <- IHt1. reflexivity.
+  Case "term_ToLabeled". simpl. rewrite <- IHt1_2. reflexivity.
+  Case "term_MkToLabeledTCB". simpl. rewrite <- IHt1_4. reflexivity.
+Qed.
+
+Hint Resolve erase_term_idempotent.
+
+Lemma pure_reduce_inv : forall l t1 t2,
+  is_l_of_t l ->
+  pure_reduce (erase_term l t1) t2 ->
+  pure_reduce_l l (erase_term l t1) (erase_term l t2).
+Proof.
+  intros l t1 t2 l_of_t H.
+  apply pure_reduce_l_step. assumption. assumption.
+Qed.
+
+Hint Resolve pure_reduce_inv.
+
+Lemma erase_term_homo_subst : forall l t1 x t2,
+  is_l_of_t l ->
+  erase_term l (tsubst_t t1 x t2) = tsubst_t (erase_term l t1) x (erase_term l t2).
+Proof. Admitted.
+
+Hint Resolve erase_term_homo_subst.
+
+Lemma erase_hole_implies_anything: forall l l1 t1,
+  is_l_of_t l ->
+  is_l_of_t l1 ->
+  canFlowTo l1 l = Some false ->
+  erase_term l (t_VLabeled l1 t_VHole) = erase_term l (t_VLabeled l1 t1).
+Proof.
+  intros. simpl. rewrite H1. simpl. reflexivity.
+Qed. 
+
+Lemma pure_reduce_simulation : forall l t1 t2,
+  is_l_of_t l ->
+  pure_reduce t1 t2 ->
+  pure_reduce_l l (erase_term l t1) (erase_term l t2).
+Proof.
+  intros l t1 t2 l_of_t H.
+  generalize dependent t2.
+  term_cases (induction t1) Case; intros t2 H.
+    Case "term_LBot". apply labels_cannot_be_reduced in H. contradiction. simpl. trivial.
+    Case "term_LA". apply labels_cannot_be_reduced in H. contradiction. simpl. trivial.
+    Case "term_LB". apply labels_cannot_be_reduced in H. contradiction. simpl. trivial.
+    Case "term_LTop". apply labels_cannot_be_reduced in H. contradiction. simpl. trivial.
+    Case "term_VTrue". apply values_cannot_be_reduced in H. contradiction. simpl. trivial.
+    Case "term_VFalse". apply values_cannot_be_reduced in H. contradiction. simpl. trivial.
+    Case "term_VUnit". apply values_cannot_be_reduced in H. contradiction. simpl. trivial.
+    Case "term_VAbs". inversion H. 
+    Case "term_VFix". inversion H.
+     SCase "fixCtx".
+     apply Pr_fixCtx in H1.
+     apply IHt1 in H1.
+     rewrite erase_term_idempotent with (t1 := t_VFix t').
+     rewrite erase_term_idempotent with (t1 := t_VFix t1).
+     assert (erase_term l (t_VFix t1) = (t_VFix (erase_term l t1))) as Hr.
+     SSCase "assert". trivial.
+     rewrite Hr.
+     apply pure_reduce_l_step. assumption.
+     apply IHt1 in H1.
+     inversion H1.
+     subst.
+     inversion H5.auto.
+
+apply Pr_fixCtx.
+     apply pure_reduce_l_step. assumption.
+     simpl.
+
+     SCase "fix".
+     rewrite erase_term_idempotent with (t1 := tsubst_t (t_VFix (t_VAbs x t5)) x t5).
+     apply pure_reduce_l_step. assumption.
+     simpl. rewrite erase_term_homo_subst.
+     apply Pr_fix. assumption. assumption.
+    Case "term_VLIO". inversion H.
+    Case "term_VLabeled". inversion H.
+    Case "term_VHole". inversion H.
+    Case "term_Var". inversion H.
+    Case "term_App".  inversion H.
+     SCase "appCtx".
+     apply IHt1_1 in H3.
+     rewrite erase_term_idempotent with (t1 := t_App t1' t1_2).
+     apply pure_reduce_l_step. assumption.
+     simpl. apply Pr_appCtx.
+     apply pure_reduce_inv_simulation. assumption. assumption. assumption.
+     SCase "app".  
+     rewrite erase_term_idempotent with (t1 := tsubst_t t1_2 x t1).
+     apply pure_reduce_l_step. assumption.
+     simpl. rewrite erase_term_homo_subst.
+     apply Pr_app. assumption. assumption.
+    Case "term_IfEl". inversion H.
+     SCase "ifCtx".
+     rewrite erase_term_idempotent with (t1 := t_IfEl t1' t1_2 t1_3).  
+     apply pure_reduce_l_step. assumption.
+     simpl. apply Pr_ifCtx. assumption. assumption.
+     SCase "ifTrue".
+     rewrite erase_term_idempotent with (t1 := t2).  
+     apply pure_reduce_l_step. assumption.
+     simpl. apply Pr_ifTrue. assumption.
+     SCase "ifFalse".
+     rewrite erase_term_idempotent with (t1 := t2).  
+     apply pure_reduce_l_step. assumption.
+     simpl. apply Pr_ifFalse. assumption.
+    Case "term_Join". simpl. apply pure_reduce_l_step. assumption. assumption.
+    Case "term_Meet". simpl. apply pure_reduce_l_step. assumption. assumption.
+    Case "term_CanFlowTo". simpl. apply pure_reduce_l_step. assumption. assumption.
+    Case "term_Return". inversion H.
+    Case "term_Bind". inversion H. 
+    Case "term_GetLabel". inversion H.
+    Case "term_GetClearance". inversion H.
+    Case "term_LabelOf". admit.
+    Case "term_Label". inversion H.
+    Case "term_UnLabel". inversion H.
+    Case "term_ToLabeled". inversion H.
+    Case "term_MkToLabeledTCB". inversion H.
+Qed.
+
+Lemma erase_config_idempotent : forall l m1,
+  is_l_of_t l ->
+  erase_config l m1 = erase_config l (erase_config l m1).
+Proof.
+  Admitted.
